Examples.lean
@@ -16,6 +16,7 @@ import Examples.Ram.Composition
 import Examples.Ram.ContractFill
 import Examples.Ram.Factorial
 import Examples.Ram.FactorialFunction
+import Examples.Ram.FactorialStream
 import Examples.Ram.FunctionRun
 import Examples.Ram.LocalBindings
 import Examples.Ram.GraphDegree
